Bound name preserving in rewrites for ExSet

Phi_Semantics/PhiSem_CF_Routine.thy
@@ -6,40 +6,42 @@ text \<open>Based on the basic routine module, we provide the version that suppo
 
 declare [[\<phi>hide_techinicals = false]]
 
-definition RETURN_FRAME :: \<open>'rets::FIX_ARITY_VALs itself \<Rightarrow> RES.brk_label \<Rightarrow> bool\<close>
-  where \<open>RETURN_FRAME _ label \<longleftrightarrow> True\<close>
+definition RETURN_FRAME :: \<open>'rets::FIX_ARITY_VALs itself \<Rightarrow> RES.brk_label \<Rightarrow> ('rets \<phi>arg \<Rightarrow> fiction set) \<Rightarrow> bool\<close>
+  where \<open>RETURN_FRAME _ label Y \<longleftrightarrow> True\<close>
+
+lemma RETURN_FRAME_I:
+  \<open> RETURN_FRAME TY label Y \<close>
+  unfolding RETURN_FRAME_def ..
 
 lemma RETURN_FRAME_normal:
-  \<open> RETURN_FRAME TYPE('rets) label
+  \<open> RETURN_FRAME TYPE('rets) label Y
 \<Longrightarrow> \<p>\<r>\<o>\<c> (op_break TYPE('any) TYPE('rets) label ret) \<lbrace> Y ret\<heavy_comma> TECHNICAL Brk_Frame label \<longmapsto> 0 \<rbrace>
     \<t>\<h>\<r>\<o>\<w>\<s> (\<lambda>_. Brking_Frame label Y) \<close>
   for ret :: \<open>'rets::FIX_ARITY_VALs \<phi>arg\<close>
   using op_break_\<phi>app .
 
 lemma RETURN_FRAME_unit:
-  \<open> RETURN_FRAME TYPE(unit) label
-\<Longrightarrow> \<p>\<r>\<o>\<c> (op_break TYPE('any) TYPE(unit) label (\<phi>arg ())) \<lbrace> Y\<heavy_comma> TECHNICAL Brk_Frame label \<longmapsto> 0 \<rbrace>
-    \<t>\<h>\<r>\<o>\<w>\<s> (\<lambda>_. Brking_Frame label (\<lambda>_::unit \<phi>arg. Y)) \<close>
-  using op_break_\<phi>app[where S=\<open>\<lambda>_::unit \<phi>arg. Y\<close>] .
+  \<open> RETURN_FRAME TYPE(unit) label Y
+\<Longrightarrow> \<p>\<r>\<o>\<c> (op_break TYPE('any) TYPE(unit) label (\<phi>arg ())) \<lbrace> Y (\<phi>arg ())\<heavy_comma> TECHNICAL Brk_Frame label \<longmapsto> 0 \<rbrace>
+    \<t>\<h>\<r>\<o>\<w>\<s> (\<lambda>_. Brking_Frame label Y) \<close>
+  using op_break_\<phi>app[where S=Y] .
 
-attribute_setup RETURN_FRAME = \<open>Scan.succeed (Thm.rule_attribute [] (fn _ => fn th =>
-                    @{thm' RETURN_FRAME_unit} RS th
-    handle THM _ => @{thm' RETURN_FRAME_normal} RS th ) )\<close>
+attribute_setup RETURN_FRAME = \<open>Scan.succeed (Thm.rule_attribute [] (fn ctxt => fn th =>
+                    th RS (Thm.transfer'' ctxt @{thm' RETURN_FRAME_unit})
+    handle THM _ => th RS (Thm.transfer'' ctxt @{thm' RETURN_FRAME_normal})) )\<close>
 
 declare [[
-  \<phi>premise_attribute [RETURN_FRAME] for \<open>RETURN_FRAME _ _\<close>  (%\<phi>attr)
+  \<phi>premise_attribute [RETURN_FRAME] for \<open>RETURN_FRAME _ _ _\<close>  (%\<phi>attr)
 ]]
 
+(* RETURN_FRAME TYPE('rets::FIX_ARITY_VALs) label_ret *)
 
 proc op_routine:
   requires Ty_X: \<open>\<phi>_Have_Types X TY_ARGs\<close>
       and  Ty_Y: \<open>\<phi>_Have_Types Y TY_RETs\<close>
       and  \<open>\<r>Success\<close>
       and  F: \<open>(\<And>(vs:: 'args::FIX_ARITY_VALs \<phi>arg <named> 'names) label_ret.
-            return_\<phi>app\<^bold>: TECHNICAL(
-                \<forall>ret :: 'rets::FIX_ARITY_VALs \<phi>arg.
-                  \<p>\<r>\<o>\<c> (op_break TYPE('rets) TYPE('rets) label_ret ret) \<lbrace> Y ret\<heavy_comma> TECHNICAL Brk_Frame label_ret \<longmapsto> 0 \<rbrace>
-                  \<t>\<h>\<r>\<o>\<w>\<s> (\<lambda>_. Brking_Frame label_ret Y))
+            return_\<phi>app\<^bold>: TECHNICAL(RETURN_FRAME TYPE('rets::FIX_ARITY_VALs) label_ret Y)
             \<Longrightarrow> \<p>\<r>\<o>\<c> F label_ret (case_named (\<lambda>x. x) vs) \<lbrace> X (case_named id vs)\<heavy_comma> TECHNICAL Brk_Frame label_ret
                                                 \<longmapsto> \<lambda>ret. Y ret\<heavy_comma> TECHNICAL Brk_Frame label_ret
                                                   \<rbrace> \<t>\<h>\<r>\<o>\<w>\<s> (\<lambda>e. \<b>\<r>\<e>\<a>\<k> label_ret \<w>\<i>\<t>\<h> Y \<o>\<r> E e))\<close>
@@ -50,21 +52,12 @@ proc op_routine:
   apply_rule "__routine_basic__"[OF Ty_X Ty_Y \<r>Success_I, where 'names='names,
                                  unfolded named_All, simplified]
   \<medium_left_bracket> for vs 
-    op_brk_scope \<medium_left_bracket> for label_ret
-      apply_rule F[of label_ret \<open>tag vs\<close>, unfolded Technical_def[where 'a=\<open>bool\<close>], simplified]
-      apply_rule op_break
+    op_brk_scope \<medium_left_bracket>  for label_ret
+      apply_rule F[of label_ret \<open>tag vs\<close>, unfolded Technical_def[where 'a=\<open>bool\<close>], simplified, OF RETURN_FRAME_I]
     \<medium_right_bracket>
   \<medium_right_bracket>
 \<medium_right_bracket> .
 
-thm op_break_\<phi>app
-
-lemma
-  \<open>\<forall>ret :: unit \<phi>arg. \<p>\<r>\<o>\<c> (op_break TYPE('rets) TYPE('rets) label_ret ret) \<lbrace> Y ret\<heavy_comma> TECHNICAL Brk_Frame label_ret \<longmapsto> 0 \<rbrace>
-                      \<t>\<h>\<r>\<o>\<w>\<s> (\<lambda>_. Brking_Frame label_ret Y)
- \<equiv> \<close>
-
-thm op_routine_\<phi>app
 
 abbreviation
   \<open>op_rec_routine argtys rettys F \<equiv> op_fix_point (\<lambda>\<f>.
@@ -77,6 +70,6 @@ attribute_setup routine =
           (fn N => fn wrap => fn Tm => Abs("label_ret", \<^typ>\<open>RES.brk_label\<close>, wrap (Tm $ Bound N)))
           @{thm "op_routine_\<phi>app"}))\<close>
 
-hide_fact RETURN_FRAME_normal
+hide_fact RETURN_FRAME_normal RETURN_FRAME_unit
 
 end
