Phi_Examples/PhiEx_Slice.thy
@@ -5,16 +5,6 @@ theory PhiEx_Slice
 begin
 
 declare One_nat_def[simp del]
-
-term sorted
-term permute_list
-
-term \<open>A <~~> B\<close>
-
-declare [[\<phi>trace_reasoning = 2]]
-declare [[\<phi>hide_techinicals = false]]
-declare [[\<phi>trace_premise_attrs = true]]
-
  
 proc qsort:
   input  \<open>l \<Ztypecolon> \<m>\<e>\<m>[addr] \<s>\<l>\<i>\<c>\<e>[i,len] \<nat>(32)\<heavy_comma>
@@ -26,23 +16,10 @@ proc qsort:
   is [recursive l addr i len]
   is [routine]
 \<medium_left_bracket>
-  thm qsort
-
-
-  note \<open>length l = len\<close>[useful] ;;
   if ($len \<le> 1)
-    \<medium_left_bracket> 
-      thm return_\<phi>app
-      \<medium_right_bracket>
-  \<medium_left_bracket> 
-
-$i + ($len-1) \<rightarrow> val tt;;
-      note [[\<phi>trace_reasoning = 2]] ;;
-
- $tt !
-
-    ;;
-val pivot \<leftarrow> ($i + ($len - 1)) ! ;;
+  \<medium_left_bracket> return \<medium_right_bracket>
+  \<medium_left_bracket>
+    val pivot \<leftarrow> ($i + ($len - 1)) ! ;;
     var d \<leftarrow> 0 ;;
     replicate (0,$len) \<open>\<lambda>n. l' \<Ztypecolon> \<m>\<e>\<m>[addr] \<s>\<l>\<i>\<c>\<e>[i,len] \<nat>(32)\<heavy_comma>
                             d \<Ztypecolon> \<v>\<a>\<r>[d] \<nat>(32)
@@ -64,67 +41,18 @@ val pivot \<leftarrow> ($i + ($len - 1)) ! ;;
     (*readers may inspect \<open>thm useful\<close> to look the contextual facts*)
     (* thm useful *)
     qsort ($i, $d) ;;
-    qsort ($i + $d, $len - $d)
+    qsort ($i + $d, $len - $d) ;;
           
-    pure_fact t1: \<open>\<forall>x\<in>set (drop d l'). l ! (len - 1) < x\<close>
+    pure_fact t1: \<open>\<forall>x\<in>set (drop d l'). l ! (len - 1) < x\<close> ;;
     pure_fact t2: \<open>\<forall>x\<in>set (take d l'). x \<le> l ! (len - 1)\<close> ;;
 
-    \<open>l' \<Ztypecolon> \<m>\<e>\<m>[addr] \<s>\<l>\<i>\<c>\<e>[i,len] \<nat>(32) \<s>\<u>\<b>\<j> l'. l <~~> l' \<and> sorted l'\<close>
+    return
 
-  \<medium_right_bracket> for \<open>l' \<Ztypecolon> \<m>\<e>\<m>[addr] \<s>\<l>\<i>\<c>\<e>[i,len] \<nat>(32) \<s>\<u>\<b>\<j> l'. l <~~> l' \<and> sorted l'\<close> ;;
+  \<medium_right_bracket>
+\<medium_right_bracket> .
 
-
-
-                      thm qsort[]
-    thm useful
-    thm qsort
-
-
-
-
-
-
-
-
-
-
-
-
-
-
-
-
-
-
-
-
-
-
-
-(*
-
-proc qsort:
-  input  \<open>l  \<Ztypecolon> \<m>\<e>\<m>[addr] \<s>\<l>\<i>\<c>\<e>[i,len] \<nat>(32)\<heavy_comma>
-          j  \<Ztypecolon> \<v>\<a>\<l> \<Ss>\<Pp>\<t>\<r>[addr:i:len] \<i>\<n>\<t>(32)\<heavy_comma>
-          len \<Ztypecolon> \<v>\<a>\<l> \<nat>(32)\<close>
-  premises \<open>j = 0\<close>
-  output \<open>l' \<Ztypecolon> \<m>\<e>\<m>[addr] \<s>\<l>\<i>\<c>\<e>[i,n] \<nat>(32) \<s>\<u>\<b>\<j> l'. l <~~> l' \<and> sorted l'\<close>
-\<medium_left_bracket>
-  if ($len \<le> 1)
-  \<medium_left_bracket> \<medium_right_bracket>
-  \<medium_left_bracket>
-    val pivot \<leftarrow> $j !;;
-    var k \<leftarrow> 1 ;;
-    while' \<open>k \<Ztypecolon> \<v>\<a>\<r>[k] \<nat>(32)\<heavy_comma>
-            low \<Ztypecolon> \<m>\<e>\<m>[addr] \<s>\<l>\<i>\<c>\<e>[i,k] \<nat>(32)\<heavy_comma>
-            up \<Ztypecolon> \<m>\<e>\<m>[addr] \<s>\<l>\<i>\<c>\<e>[i+k,len-k] \<nat>(32)
-            \<s>\<u>\<b>\<j> k low up. Inv: (k \<le> )
-                        \<and> Guard: ()\<close>
-
-*)
-
-
-
+thm qsort_def   \<comment> \<open>semantic representation of \<open>qsort\<close>\<close>
+thm qsort_\<phi>app \<comment> \<open>specification theorem\<close>
 
 
 end
